core/Protobuf.v
@@ -34,63 +34,20 @@ Inductive LockservTag :=
 | UnlockTag
 | LockedTag.
 
-Definition LockservTag_sm : unit -> (byte -> fold_state unit LockservTag) + LockservTag :=
-  fun _ => inl (fun b => match b with
-                         | x00 => Done LockTag
-                         | x01 => Done UnlockTag
-                         | x02 => Done LockedTag
-                         | _ => Error
-                         end).
-
-
-Parameter nat_sm_t : Type.
-Parameter nat_sm_step : byte -> nat_sm_t -> fold_state nat_sm_t nat.
-Parameter nat_sm_init : nat_sm_t.
-
-Definition nat_sm_step' : nat_sm_t -> (byte -> fold_state nat_sm_t nat) + nat :=
-  fun ns => inl (fun b => nat_sm_step b ns).
-
-Inductive lockserv_sm_t :=
-| Tag
-| Body : LockservTag * nat_sm_t -> lockserv_sm_t.
-
-Definition LocskervMsg_deserialize_manual
-           (b : byte)
-           (s: lockserv_sm_t) : fold_state lockserv_sm_t LockservMsg :=
-  match s with
-  | Tag => match b with
-           | x00 => More (Body (LockTag, nat_sm_init))
-           | x01 => Done Unlock
-           | x02 => More (Body (LockedTag, nat_sm_init))
-           | _ => Error
-           end
-  | Body (t, ns) => match nat_sm_step b ns with
-                    | Done n => match t with
-                                | LockTag => Done (Lock n)
-                                | UnlockTag => Error
-                                | LockedTag => Done (Locked n)
-                                end
-                    | More ns => More (Body (t, ns))
-                    | Error => Error
-                    end
-  end.
-
-Definition Lockserv_tag_sm : unit -> (byte -> fold_state unit LockservTag) + LockservTag :=
-  fun _ => inl (fun b => match b with
-                         | x00 => Done LockTag
-                         | x01 => Done UnlockTag
-                         | x02 => Done LockedTag
-                         | _ => Error
-                         end).
-
-Definition Lockserv_body_sm (t : LockservTag) (s : nat_sm_t + (nat * unit))
-  : (byte -> fold_state (nat_sm_t + nat * unit) LockservMsg) + LockservMsg :=
-    match t with
-    | LockTag =>  inr Unlock
-    | UnlockTag => inr Unlock
-    | LockedTag => inr Unlock
+Definition LockservMsg_deserialize_tag : state_machine unit LockservTag :=
+  fun (byte : byte) _ =>
+    match byte with
+    | x00 => Done LockTag
+    | x01 => Done UnlockTag
+    | x02 => Done LockedTag
+    | _ => Error
     end.
 
-Definition lockserv_deserialize :=
-  ByteListReader.bind_sm Lockserv_tag_sm
-                         Lockserv_body_sm.
+Definition LockservMsg_deserialize_tag_value :=
+  ByteListReader.bind_sm LockservMsg_deserialize_tag
+                         (fun tag => match tag with
+                                     | LockTag => fun b _ => Done (Lock (byte_to_nat b))
+                                     | UnlockTag => fun _ _ => Done Unlock
+                                     | LockedTag => fun b _ => Done (Locked (byte_to_nat b))
+                                     end)
+                         (fun _ => tt).
